L3_Model/arm-vfp.spec
@@ -1,0 +1,658 @@
+-----------------------------------------------------------------------
+-- Formal Specification of the ARMv7-AR instruction set architecture --
+-- Floating-point specification for VFPv4-D32                        --
+-- (c) Anthony Fox, University of Cambridge                          --
+-----------------------------------------------------------------------
+
+-------------------------------------------------------------------------
+-- NOTE: This specification is incomplete.
+-- In particular, it does not attempt to properly model the behaviour
+-- of exceptions and NaNs. Also skips fixed-point instructions.
+-------------------------------------------------------------------------
+
+type dreg  = bits(5)
+
+construct VFPExtension {
+   NoVFP
+   VFPv2
+   VFPv3
+   VFPv4
+}
+
+declare VFPExtension :: VFPExtension
+
+---------------------------------------------
+-- Floating-point and Advanced SIMD registers
+---------------------------------------------
+
+-- Floating-point Status and Control Register (PMSA)
+
+register FPSCR :: word {
+   31:    N     -- Condition flag (Negative)
+   30:    Z     -- Condition flag (Zero)
+   29:    C     -- Condition flag (Carry)
+   28:    V     -- Condition flag (oVerflow)
+   27:    QC    -- Cumulative saturation bit, Advanced SIMD only
+   26:    AHP   -- Alternative half-precision control bit
+   25:    DN    -- Default NaN mode control bit
+   24:    FZ    -- Flush-to-zero mode control bit
+   23-22: RMode -- Rounding mode: 00 - RN, 01 - RP, 10 - RM, 11 - RZ
+   21-20: RAZ!  -- previously Stride
+   19:    RAZ!  -- Reserved
+   18-16: RAZ!  -- previously Len
+   15:    IDE   -- Input Denormal exception trap enable
+   14-13: RAZ!  -- Reserved
+   12:    IXE   -- Inexact exception trap enable
+   11:    UFE   -- Underflow exception trap enable
+   10:    OFE   -- Overflow exception trap enable
+   9:     DZE   -- Division by Zero exception trap enable
+   8:     IOE   -- Invalid Operation exception trap enable
+   7:     IDC   -- Input Denormal cumulative exception bit
+   6-5:   RAZ!  -- Reserved
+   4:     IXC   -- Inexact cumulative exception bit
+   3:     UFC   -- Underflow cumulative exception bit
+   2:     OFC   -- Overflow cumulative exception bit
+   1:     DZC   -- Division by Zero cumulative exception bit
+   0:     IOC   -- Invalid Operation cumulative exception bit
+}
+
+record FP {
+   REG :: dreg -> dword  -- 32 64-bit registers (D32)
+                         -- Some processors will only have 16 registers
+                         -- e.g. VFPv2, VFPv3-D16.
+   FPSCR :: FPSCR
+}
+
+declare FP :: FP
+
+--------------------
+-- Helper Operations
+--------------------
+
+exception VFP_EXCEPTION :: string
+
+ieee_rounding RoundingMode =
+   match FP.FPSCR.RMode
+   {
+      case '00' => roundTiesToEven
+      case '01' => roundTowardPositive
+      case '10' => roundTowardNegative
+      case '11' => roundTowardZero
+   }
+
+word FPAdd32 (op1::word, op2::word) = FP32_Add (RoundingMode, op1, op2)
+word FPSub32 (op1::word, op2::word) = FP32_Sub (RoundingMode, op1, op2)
+word FPMul32 (op1::word, op2::word) = FP32_Mul (RoundingMode, op1, op2)
+
+dword FPAdd64 (op1::dword, op2::dword) = FP64_Add (RoundingMode, op1, op2)
+dword FPSub64 (op1::dword, op2::dword) = FP64_Sub (RoundingMode, op1, op2)
+dword FPMul64 (op1::dword, op2::dword) = FP64_Mul (RoundingMode, op1, op2)
+
+word FPToFixed32 (operand::word, unsigned::bool, round_towards_zero::bool) =
+{
+  mode = if round_towards_zero then roundTowardZero else RoundingMode;
+  match FP32_ToInt (mode, operand)
+  {
+    case Some (i) =>
+      { result, overflow = SatQ (i, 32, unsigned);
+        if overflow then
+           -- L3 model does not cover VFP exceptions
+           #VFP_EXCEPTION "FPToFixed32: overflow exception"
+        else
+           result
+      }
+    case None => #VFP_EXCEPTION "FPToFixed32: NaN or infinity"
+  }
+}
+
+word FPToFixed64 (operand::dword, unsigned::bool, round_towards_zero::bool) =
+{
+  mode = if round_towards_zero then roundTowardZero else RoundingMode;
+  match FP64_ToInt (mode, operand)
+  {
+    case Some (i) =>
+      { result, overflow = SatQ (i, 32, unsigned);
+        if overflow then
+           -- L3 model does not cover VFP exceptions
+           #VFP_EXCEPTION "FPToFixed64: overflow exception"
+        else
+           result
+      }
+    case None => #VFP_EXCEPTION "FPToFixed64: NaN or infinity"
+  }
+}
+
+word FixedToFP32 (operand::word, unsigned::bool, round_to_nearest::bool) =
+{
+  mode = if round_to_nearest then roundTiesToEven else RoundingMode;
+  int_operand = if unsigned then [[operand]::nat] else [operand];
+  FP32_FromInt (mode, int_operand)
+}
+
+dword FixedToFP64 (operand::word, unsigned::bool, round_to_nearest::bool) =
+{
+  mode = if round_to_nearest then roundTiesToEven else RoundingMode;
+  int_operand = if unsigned then [[operand]::nat] else [operand];
+  FP64_FromInt (mode, int_operand)
+}
+
+component D (n::dreg) :: dword
+{
+  value = FP.REG (n)
+  assign value = FP.REG (n) <- value
+}
+
+component S (n::dreg) :: word
+{
+  value = if n<0> then D(n div 2)<63:32> else D(n div 2)<31:0>
+  assign value = if n<0> then
+                    D(n div 2)<63:32> <- value
+                 else
+                    D(n div 2)<31:0> <- value
+}
+
+dword VFPExpandImm (imm8::byte, single::bool) =
+   if single then
+      ZeroExtend (imm8<7:7> : ~imm8<6:6> : imm8<6:6> ^ 5 : imm8<5:0> : '0' ^ 19)
+   else
+      imm8<7:7> : ~imm8<6:6> : imm8<6:6> ^ 8 : imm8<5:0> : '0' ^ 48
+
+bits(4) FPCompare32 (op1::word, op2::word) =
+   if FP32_IsNan (op1) or FP32_IsNan (op2) then
+      '0011'
+   else if FP32_Equal (op1, op2) then
+      '0110'
+   else if FP32_LessThan (op1, op2) then
+      '1000'
+   else
+      '0010'
+
+bits(4) FPCompare64 (op1::dword, op2::dword) =
+   if FP64_IsNan (op1) or FP64_IsNan (op2) then
+      '0011'
+   else if FP64_Equal (op1, op2) then
+      '0110'
+   else if FP64_LessThan (op1, op2) then
+      '1000'
+   else
+      '0010'
+
+bits(32) FPZero32 (sign::bits(1)) = sign : 0`31
+bits(64) FPZero64 (sign::bits(1)) = sign : 0`63
+
+------------------------
+-- Instruction Semantics
+------------------------
+
+-- ~~~~~~~~~~~~~~~~~~~~~~~~~~~~
+-- VMOV<c>.F64 <Dd>, #<imm>
+-- VMOV<c>.F32 <Sd>, #<imm>
+-- ~~~~~~~~~~~~~~~~~~~~~~~~~~~~
+define VFP > vmov_imm (single_register::bool, d::dreg, imm64::dword) =
+{
+   if single_register then
+      S(d) <- imm64<31:0>
+   else
+      D(d) <- imm64;
+   IncPC()
+}
+
+-- ~~~~~~~~~~~~~~~~~~~~~~~~~~~~
+-- VMOV<c>.F64 <Dd>, <Dm>
+-- VMOV<c>.F32 <Sd>, <Sm>
+-- ~~~~~~~~~~~~~~~~~~~~~~~~~~~~
+define VFP > vmov (single_register::bool, d::dreg, m::dreg) =
+{
+   if single_register then
+      S(d) <- S(m)
+   else
+      D(d) <- D(m);
+   IncPC()
+}
+
+-- ~~~~~~~~~~~~~~~~~~~~~~~~~~~~
+-- VMOV<c> <Sn>, <Rt>
+-- VMOV<c> <Rt>, <Sn>
+-- ~~~~~~~~~~~~~~~~~~~~~~~~~~~~
+define VFP > vmov_single (to_arm_register::bool, t::reg, n::dreg) =
+{
+   if to_arm_register then
+      R(t) <- S(n)
+   else
+      S(n) <- R(t);
+   IncPC()
+}
+
+-- ~~~~~~~~~~~~~~~~~~~~~~~~~~~~~~~~
+-- VMOV<c> <Sm>, <Sm1>, <Rt>, <Rt2>
+-- VMOV<c> <Rt>, <Rt2>, <Sm>, <Sm1>
+-- ~~~~~~~~~~~~~~~~~~~~~~~~~~~~~~~~
+define VFP > vmov_two_singles
+  (to_arm_registers::bool, t::reg, t2::reg, m::dreg) =
+{
+   if to_arm_registers then
+   {
+      R(t) <- S(m);
+      R(t2) <- S(m+1)
+   }
+   else
+   {
+      S(m) <- R(t);
+      S(m+1) <- R(t2)
+   };
+   IncPC()
+}
+
+-- ~~~~~~~~~~~~~~~~~~~~~~~~~~~~~~~~
+-- VMOV<c> <Dm>, <Rt>, <Rt2>
+-- VMOV<c> <Rt>, <Rt2>, <Dm>
+-- ~~~~~~~~~~~~~~~~~~~~~~~~~~~~~~~~
+define VFP > vmov_double
+  (to_arm_registers::bool, t::reg, t2::reg, m::dreg) =
+{
+   if to_arm_registers then
+   {
+      R(t) <- D(m)<31:0>;
+      R(t2) <- D(m)<63:32>
+   }
+   else
+   {
+      D(m)<31:0> <- R(t);
+      D(m)<63:32> <- R(t2)
+   };
+   IncPC()
+}
+
+-- ~~~~~~~~~~~~~~~~~~~~~~~~~~~~
+-- VABS<c>.F64 <Dd>, <Dm>
+-- VABS<c>.F32 <Sd>, <Sm>
+-- ~~~~~~~~~~~~~~~~~~~~~~~~~~~~
+define VFP > vabs (dp_operation::bool, d::dreg, m::dreg) =
+{
+   if dp_operation then
+      D(d) <- FP64_Abs (D(m))
+   else
+      S(d) <- FP32_Abs (S(m));
+   IncPC()
+}
+
+-- ~~~~~~~~~~~~~~~~~~~~~~~~~~~~
+-- VNEG<c>.F64 <Dd>, <Dm>
+-- VNEG<c>.F32 <Sd>, <Sm>
+-- ~~~~~~~~~~~~~~~~~~~~~~~~~~~~
+define VFP > vneg (dp_operation::bool, d::dreg, m::dreg) =
+{
+   if dp_operation then
+      D(d) <- FP64_Neg (D(m))
+   else
+      S(d) <- FP32_Neg (S(m));
+   IncPC()
+}
+
+-- ~~~~~~~~~~~~~~~~~~~~~~~~~~~~
+-- VSQRT<c>.F64 <Dd>, <Dm>
+-- VSQRT<c>.F32 <Sd>, <Sm>
+-- ~~~~~~~~~~~~~~~~~~~~~~~~~~~~
+define VFP > vsqrt (dp_operation::bool, d::dreg, m::dreg) =
+{
+   if dp_operation then
+      D(d) <- FP64_Sqrt (RoundingMode, D(m))
+   else
+      S(d) <- FP32_Sqrt (RoundingMode, S(m));
+   IncPC()
+}
+
+-- ~~~~~~~~~~~~~~~~~~~~~~~~~~~~~~
+-- VCVT<c>.F64.F32 <Dd>, <Sm>
+-- VCVT<c>.F32.F64 <Sd>, <Dm>
+-- ~~~~~~~~~~~~~~~~~~~~~~~~~~~~~~
+define VFP > vcvt_float (double_to_single::bool, d::dreg, m::dreg) =
+{
+   if double_to_single then
+      S(d) <- FP64_ToFP32 (RoundingMode, D(m))
+   else
+      D(d) <- FP32_ToFP64 (S(m));
+   IncPC()
+}
+
+-- ~~~~~~~~~~~~~~~~~~~~~~~~~~~~~~
+-- VCVT{R}<c>.S32.F64 <Sd>, <Dm>
+-- VCVT{R}<c>.S32.F32 <Sd>, <Sm>
+-- VCVT{R}<c>.U32.F64 <Sd>, <Dm>
+-- VCVT{R}<c>.U32.F32 <Sd>, <Sm>
+-- ~~~~~~~~~~~~~~~~~~~~~~~~~~~~~~
+define VFP > vcvt_to_integer
+  (dp_operation::bool, unsigned::bool, round_zero::bool, d::dreg, m::dreg) =
+{
+   if dp_operation then
+      S(d) <- FPToFixed64 (D(m), unsigned, round_zero)
+   else
+      S(d) <- FPToFixed32 (S(m), unsigned, round_zero);
+   IncPC()
+}
+
+-- ~~~~~~~~~~~~~~~~~~~~~~~~~~~~~~
+-- VCVT<c>.F64.S32 <Dd>, <Sm>
+-- VCVT<c>.F64.U32 <Dd>, <Sm>
+-- VCVT<c>.F32.S32 <Sd>, <Sm>
+-- VCVT<c>.F32.U32 <Sd>, <Sm>
+-- ~~~~~~~~~~~~~~~~~~~~~~~~~~~~~~
+define VFP > vcvt_from_integer
+  (dp_operation::bool, unsigned::bool, d::dreg, m::dreg) =
+{
+   if dp_operation then
+      D(d) <- FixedToFP64 (S(m), unsigned, false)
+   else
+      S(d) <- FixedToFP32 (S(m), unsigned, false);
+   IncPC()
+}
+
+-- ~~~~~~~~~~~~~~~~~~~~~~~~~~~~
+-- VCMP{E}<c>.F64 <Dd>, <Dm>
+-- VCMP{E}<c>.F64 <Dd>, #0.0
+-- VCMP{E}<c>.F32 <Sd>, <Sm>
+-- VCMP{E}<c>.F32 <Sd>, #0.0
+-- ~~~~~~~~~~~~~~~~~~~~~~~~~~~~
+define VFP > vcmp (dp_operation::bool, d::dreg, m_with_zero::dreg option) =
+{
+   if dp_operation then
+   {
+      op2 = match m_with_zero
+            {
+               case Some (m) => D(m)
+               case None => FPZero64 ('0')
+            };
+      FP.&FPSCR<31:28> <- FPCompare64 (D(d), op2)
+   }
+   else
+   {
+      op2 = match m_with_zero
+            {
+               case Some (m) => S(m)
+               case None => FPZero32 ('0')
+            };
+      FP.&FPSCR<31:28> <- FPCompare32 (S(d), op2)
+   };
+   IncPC()
+}
+
+-- ~~~~~~~~~~~~~~~~~~~~~~~~~~~~
+-- VMSR<c> FPSCR, <Rt>
+-- ~~~~~~~~~~~~~~~~~~~~~~~~~~~~
+define VFP > vmsr (t::reg) =
+{
+   FP.&FPSCR <- R(t);
+   IncPC()
+}
+
+-- ~~~~~~~~~~~~~~~~~~~~~~~~~~~~
+-- VMRS<c> <Rt>, FPSCR
+-- ~~~~~~~~~~~~~~~~~~~~~~~~~~~~
+define VFP > vmrs (t::reg) =
+{
+   if t != 15 then
+      R(t) <- FP.&FPSCR
+   else
+   {
+      CPSR.N <- FP.FPSCR.N;
+      CPSR.Z <- FP.FPSCR.Z;
+      CPSR.C <- FP.FPSCR.C;
+      CPSR.V <- FP.FPSCR.V
+   };
+   IncPC()
+}
+
+-- ~~~~~~~~~~~~~~~~~~~~~~~~~~~~
+-- VADD<c>.F64 <Dd>, <Dn>, <Dm>
+-- VADD<c>.F32 <Sd>, <Sn>, <Sm>
+-- ~~~~~~~~~~~~~~~~~~~~~~~~~~~~
+define VFP > vadd (dp_operation::bool, d::dreg, n::dreg, m::dreg) =
+{
+   if dp_operation then
+      D(d) <- FPAdd64 (D(n), D(m))
+   else
+      S(d) <- FPAdd32 (S(n), S(m));
+   IncPC()
+}
+
+-- ~~~~~~~~~~~~~~~~~~~~~~~~~~~~
+-- VSUB<c>.F64 <Dd>, <Dn>, <Dm>
+-- VSUB<c>.F32 <Sd>, <Sn>, <Sm>
+-- ~~~~~~~~~~~~~~~~~~~~~~~~~~~~
+define VFP > vsub (dp_operation::bool, d::dreg, n::dreg, m::dreg) =
+{
+   if dp_operation then
+      D(d) <- FPSub64 (D(n), D(m))
+   else
+      S(d) <- FPSub32 (S(n), S(m));
+   IncPC()
+}
+
+-- ~~~~~~~~~~~~~~~~~~~~~~~~~~~~
+-- VMUL<c>.F64 <Dd>, <Dn>, <Dm>
+-- VMUL<c>.F32 <Sd>, <Sn>, <Sm>
+-- ~~~~~~~~~~~~~~~~~~~~~~~~~~~~
+define VFP > vmul (dp_operation::bool, d::dreg, n::dreg, m::dreg) =
+{
+   if dp_operation then
+      D(d) <- FPMul64 (D(n), D(m))
+   else
+      S(d) <- FPMul32 (S(n), S(m));
+   IncPC()
+}
+
+-- ~~~~~~~~~~~~~~~~~~~~~~~~~~~~
+-- VDIV<c>.F64 <Dd>, <Dn>, <Dm>
+-- VDIV<c>.F32 <Sd>, <Sn>, <Sm>
+-- ~~~~~~~~~~~~~~~~~~~~~~~~~~~~
+define VFP > vdiv (dp_operation::bool, d::dreg, n::dreg, m::dreg) =
+{
+   if dp_operation then
+      D(d) <- FP64_Div (RoundingMode, D(n), D(m))
+   else
+      S(d) <- FP32_Div (RoundingMode, S(n), S(m));
+   IncPC()
+}
+
+-- ~~~~~~~~~~~~~~~~~~~~~~~~~~~~
+-- VMLA<c>.F64 <Dd>, <Dn>, <Dm>
+-- VMLA<c>.F32 <Sd>, <Sn>, <Sm>
+-- VMLS<c>.F64 <Dd>, <Dn>, <Dm>
+-- VMLS<c>.F32 <Sd>, <Sn>, <Sm>
+-- ~~~~~~~~~~~~~~~~~~~~~~~~~~~~
+define VFP > vmla_vmls
+   (dp_operation::bool, add::bool, d::dreg, n::dreg, m::dreg) =
+{
+   if dp_operation then
+   {
+      product = FPMul64 (D(n), D(m));
+      addend = if add then product else FP64_Neg (product);
+      D(d) <- FPAdd64 (D(n), addend)
+   }
+   else
+   {
+      product = FPMul32 (S(n), S(m));
+      addend = if add then product else FP32_Neg (product);
+      S(d) <- FPAdd32 (S(n), addend)
+   };
+   IncPC()
+}
+
+-- ~~~~~~~~~~~~~~~~~~~~~~~~~~~~
+-- VFMA<c>.F64 <Dd>, <Dn>, <Dm>
+-- VFMA<c>.F32 <Sd>, <Sn>, <Sm>
+-- VFMS<c>.F64 <Dd>, <Dn>, <Dm>
+-- VFMS<c>.F32 <Sd>, <Sn>, <Sm>
+-- ~~~~~~~~~~~~~~~~~~~~~~~~~~~~
+define VFP > vfma_vfms
+   (dp_operation::bool, add::bool, d::dreg, n::dreg, m::dreg) =
+{
+   if dp_operation then
+   {
+      op64 = D(n);
+      op64 = if add then op64 else FP64_Neg (op64);
+      D(d) <- FP64_MulAdd (RoundingMode, op64, D(m), D(d))
+   }
+   else
+   {
+      op32 = S(n);
+      op32 = if add then op32 else FP32_Neg (op32);
+      S(d) <- FP32_MulAdd (RoundingMode, op32, S(m), S(d))
+   };
+   IncPC()
+}
+
+-- ~~~~~~~~~~~~~~~~~~~~~~~~~~~~
+-- VFNMA<c>.F64 <Dd>, <Dn>, <Dm>
+-- VFNMA<c>.F32 <Sd>, <Sn>, <Sm>
+-- VFNMS<c>.F64 <Dd>, <Dn>, <Dm>
+-- VFNMS<c>.F32 <Sd>, <Sn>, <Sm>
+-- ~~~~~~~~~~~~~~~~~~~~~~~~~~~~
+define VFP > vfnma_vfnms
+   (dp_operation::bool, add::bool, d::dreg, n::dreg, m::dreg) =
+{
+   if dp_operation then
+   {
+      op64 = D(n);
+      op64 = if add then op64 else FP64_Neg (op64);
+      D(d) <- FP64_MulAdd (RoundingMode, op64, D(m), FP64_Neg (D(d)))
+   }
+   else
+   {
+      op32 = S(n);
+      op32 = if add then op32 else FP32_Neg (op32);
+      S(d) <- FP32_MulAdd (RoundingMode, op32, S(m), FP32_Neg (S(d)))
+   };
+   IncPC()
+}
+
+construct VFPNegMul {VFPNegMul_VNMLA, VFPNegMul_VNMLS, VFPNegMul_VNMUL}
+
+-- ~~~~~~~~~~~~~~~~~~~~~~~~~~~~~
+-- VNMUL<c>.F64 <Dd>, <Dn>, <Dm>
+-- VNMUL<c>.F32 <Sd>, <Sn>, <Sm>
+-- VNMLA<c>.F64 <Dd>, <Dn>, <Dm>
+-- VNMLA<c>.F32 <Sd>, <Sn>, <Sm>
+-- VNMLS<c>.F64 <Dd>, <Dn>, <Dm>
+-- VNMLS<c>.F32 <Sd>, <Sn>, <Sm>
+-- ~~~~~~~~~~~~~~~~~~~~~~~~~~~~~
+define VFP > vneg_mul
+   (dp_operation::bool, typ::VFPNegMul, d::dreg, n::dreg, m::dreg) =
+{
+   if dp_operation then
+   {
+      product = FPMul64 (D(n), D(m));
+      match typ
+      {
+         case VFPNegMul_VNMLA =>
+            D(d) <- FPAdd64 (FP64_Neg (D(d)), FP64_Neg (product))
+         case VFPNegMul_VNMLS => D(d) <- FPAdd64 (FP64_Neg (D(d)), product)
+         case VFPNegMul_VNMUL => D(d) <- FP64_Neg (product)
+      }
+   }
+   else
+   {
+      product = FPMul32 (S(n), S(m));
+      match typ
+      {
+         case VFPNegMul_VNMLA =>
+            S(d) <- FPAdd32 (FP32_Neg (S(d)), FP32_Neg (product))
+         case VFPNegMul_VNMLS => S(d) <- FPAdd32 (FP32_Neg (S(d)), product)
+         case VFPNegMul_VNMUL => S(d) <- FP32_Neg (product)
+      }
+   };
+   IncPC()
+}
+
+-- ~~~~~~~~~~~~~~~~~~~~~~~~~~~~~~~~~
+-- VLDR<c> <Dd>, [<Rn>{, #+/-<imm>}]
+-- VLDR<c> <Sd>, [<Rn>{, #+/-<imm>}]
+-- VLDR<c> <Dd>, <label>
+-- VLDR<c> <Sd>, <label>
+-- ~~~~~~~~~~~~~~~~~~~~~~~~~~~~~~~~~
+define VFP > vldr (single_reg::bool, add::bool, d::dreg, n::reg, imm32::word) =
+{
+   base = if n == 15 then Align(PC, 4) else R(n);
+   address = if add then base + imm32 else base - imm32;
+   if single_reg then
+      S(d) <- MemA (address, 4)
+   else
+   {
+      word1 = MemA (address, 4) :: word;
+      word2 = MemA (address + 4, 4) :: word;
+      D(d) <- if BigEndian() then word1:word2 else word2:word1
+   };
+   IncPC()
+}
+
+-- ~~~~~~~~~~~~~~~~~~~~~~~~~~~~~~~~~
+-- VSTR<c> <Dd>, [<Rn>{, #+/-<imm>}]
+-- VSTR<c> <Sd>, [<Rn>{, #+/-<imm>}]
+-- ~~~~~~~~~~~~~~~~~~~~~~~~~~~~~~~~~
+define VFP > vstr (single_reg::bool, add::bool, d::dreg, n::reg, imm32::word) =
+{
+   address = if add then R(n) + imm32 else R(n) - imm32;
+   if single_reg then
+      MemA (address, 4) <- S(d)
+   else
+   {
+      word = D(d);
+      MemA (address, 4) <- if BigEndian() then word<63:32> else word<31:0>;
+      MemA (address + 4, 4) <- if BigEndian() then word<31:0> else word<63:32>
+   };
+   IncPC()
+}
+
+-- ~~~~~~~~~~~~~~~~~~~~~~~~~~~~~~~~~~~~~~~~
+-- VLDM{IA|DB}<c>{.<size>} <Rn>{!}, <list>
+-- VPOP<c>{.<size>} <list>
+-- ~~~~~~~~~~~~~~~~~~~~~~~~~~~~~~~~~~~~~~~~
+define VFP > vldm
+   (single_regs::bool, add::bool, wback::bool, d::dreg, n::reg, imm8::byte) =
+{
+   imm32 = ZeroExtend (imm8 : '00');
+   regs = if single_regs then [imm8] else [imm8] div 0n2;
+   var address = if add then R(n) else R(n) - imm32;
+   for r in 0 .. regs - 1 do
+      if single_regs then
+      {
+         S(d + [r]) <- MemA(address, 4);
+         address <- address + 4
+      }
+      else
+      {
+         word1 = MemA(address, 4) :: word;
+         word2 = MemA(address + 4, 4) :: word;
+         address <- address + 8;
+         D(d + [r]) <- if BigEndian() then word1 : word2 else word2 : word1
+      };
+   when wback do R(n) <- if add then R(n) + imm32 else R(n) - imm32;
+   IncPC()
+}
+
+-- ~~~~~~~~~~~~~~~~~~~~~~~~~~~~~~~~~~~~~~~~
+-- VSTM{IA|DB}<c>{.<size>} <Rn>{!}, <list>
+-- VPUSH<c>{.<size>} <list>
+-- ~~~~~~~~~~~~~~~~~~~~~~~~~~~~~~~~~~~~~~~~
+define VFP > vstm
+   (single_regs::bool, add::bool, wback::bool, d::dreg, n::reg, imm8::byte) =
+{
+   imm32 = ZeroExtend (imm8 : '00');
+   regs = if single_regs then [imm8] else [imm8] div 0n2;
+   var address = if add then R(n) else R(n) - imm32;
+   for r in 0 .. regs - 1 do
+      if single_regs then
+      {
+         MemA(address, 4) <- S(d + [r]);
+         address <- address + 4
+      }
+      else
+      {
+         d = D(d + [r]);
+         MemA(address, 4) <- if BigEndian() then d<63:32> else d<31:0>;
+         MemA(address + 4, 4) <- if BigEndian() then d<31:0> else d<63:32>;
+         address <- address + 8
+      };
+   when wback do R(n) <- if add then R(n) + imm32 else R(n) - imm32;
+   IncPC()
+}
